src/asn1/ASN1.Spec.TLV.Specialized.fst
@@ -8,408 +8,244 @@ open ASN1.Spec.NULL
 open ASN1.Spec.OCTET_STRING
 open LowParse.Bytes
 
-module U32 = FStar.UInt32
+module I = FStar.Integers
 
-/// Specialized ASN.1 DER (Primitive) TLV Parser
-/// NOTE: For each Tag-Length-Value tuple, we firstly parse the
-///       (Tag, Length) pair as the `parser_tag`, then use it to
-///       choose a proper Value parser to parse the value.
+let parse_asn1_TLV_kind_of_type
+  (_a: asn1_primitive_type)
+: parser_kind
+= match _a with
+  | BOOLEAN      -> parse_asn1_boolean_TLV_kind
+  | NULL         -> parse_asn1_null_TLV_kind
+  | OCTET_STRING -> parse_asn1_octet_string_TLV_kind
 
+let parse_asn1_TLV_of_type
+  (_a: asn1_primitive_type)
+: parser (parse_asn1_TLV_kind_of_type _a) (datatype_of_asn1_type _a)
+= match _a with
+  | BOOLEAN      -> parse_asn1_boolean_TLV
+  | NULL         -> parse_asn1_null_TLV
+  | OCTET_STRING -> parse_asn1_octet_string_TLV
 
-/// Parser filter for valid ASN.1 DER `Tag`, `Length` pair
-let filter_the_TL
-  (a: asn1_primitive_type)
-  (x: the_asn1_type a * asn1_int32)
-: GTot bool
-= let a', len = x in
-  let min, max = bound_of_asn1_type a' in
-  asn1_length_inbound (U32.v len) min max
+let serialize_asn1_TLV_of_type
+  (_a: asn1_primitive_type)
+: serializer (parse_asn1_TLV_of_type _a)
+= match _a with
+  | BOOLEAN      -> serialize_asn1_boolean_TLV
+  | NULL         -> serialize_asn1_null_TLV
+  | OCTET_STRING -> serialize_asn1_octet_string_TLV
 
-/// Parser for valid ASN.1 DER `Tag`, `Length` pair
+/// Ad-hoc sequence parser/serializer
 ///
-let parse_the_TL
-  (a: asn1_primitive_type)
-= parse_the_asn1_tag a
+
+let parse_asn1_sequence_TL_kind
+: parser_kind
+= parse_asn1_tag_kind
+  `and_then_kind`
+  parse_asn1_length_kind_of_tag SEQUENCE
+
+let parse_asn1_sequence_TL
+: parser parse_asn1_sequence_TL_kind (the_asn1_type SEQUENCE & asn1_int32_of_tag SEQUENCE)
+= parse_the_asn1_tag SEQUENCE
   `nondep_then`
-  parse_asn1_length
-  `parse_filter`
-  filter_the_TL a
+  parse_asn1_length_of_tag SEQUENCE
 
-let parse_the_TL_unfold
-  (a: asn1_primitive_type)
-  (input: bytes)
-: Lemma (
-  let res = parse (parse_the_TL a) input in
-  match parse (parse_the_asn1_tag a) input with
-  | None -> res == None
-  | Some (a, consumed_a) ->
-    (let input_len = Seq.slice input consumed_a (Seq.length input) in
-     match parse parse_asn1_length input_len with
-     | None -> res == None
-     | Some (len, consumed_len) ->
-       (if filter_the_TL a (a, len) then
-        ( res == Some ((a, len), consumed_a + consumed_len) )
-        else
-        ( res == None ))))
-= nondep_then_eq
-  (* p1 *) (parse_the_asn1_tag a)
-  (* p2 *) (parse_asn1_length)
-  (* in *) (input);
-  parse_filter_eq
-  (* p  *) (parse_the_asn1_tag a
-           `nondep_then`
-            parse_asn1_length)
-  (* f  *) (filter_the_TL a)
-  (* in *) (input)
-
-/// Serializer for valid ASN.1 DER `Tag`, `Length` pair
-///
-let serialize_the_TL
-  (a: asn1_primitive_type)
-: serializer (parse_the_TL a)
-= serialize_the_asn1_tag a
+let serialize_asn1_sequence_TL
+: serializer parse_asn1_sequence_TL
+= serialize_the_asn1_tag SEQUENCE
   `serialize_nondep_then`
   serialize_asn1_length
-  `serialize_filter`
-  filter_the_TL a
 
-let serialize_the_TL_unfold
-  (a: asn1_primitive_type)
-  (x: parse_filter_refine (filter_the_TL a))
+#push-options "--query_stats --z3rlimit 32"
+let safe_add
+  (a b: option asn1_int32)
+: Tot (option asn1_int32)
+= let open FStar.Integers in
+  if (Some?a && Some? b && (Some?.v a) <= asn1_int32_max - (Some?.v b)) then
+  ( Some (Some?.v a + Some?.v b) )
+  else
+  ( None )
+
+let len_of_asn1_primitive_TLV
+  (#_a: asn1_primitive_type)
+  (data: datatype_of_asn1_type _a)
+: Tot (option asn1_int32)
+= let data_len = len_of_asn1_data _a data in
+  let len_len = len_of_asn1_length data_len in
+  let res = 1ul in
+  Some 1ul `safe_add` Some len_len `safe_add` Some data_len
+
+let parse_exact_bare
+  (#k: parser_kind)
+  (#t: Type0)
+  (p: parser k t)
+  (l: nat)
+: Tot (bare_parser t)
+= fun (input: bytes) ->
+  if (Seq.length input < l) then
+  ( None )
+  else
+  ( match parse p (Seq.slice input 0 l) with
+    | Some (v, n) -> if n = l then
+                     ( Some (v, (l <: consumed_length input)) )
+                     else
+                     ( None )
+    | None        -> None )
+
+let parse_exact_bare_injective_prf
+  (#k: parser_kind)
+  (#t: Type0)
+  (p: parser k t)
+  (l: nat)
+  (input1: bytes)
+  (input2: bytes)
+: Lemma
+  (requires (injective_precond (parse_exact_bare p l) input1 input2))
+  (ensures (injective_postcond (parse_exact_bare p l) input1 input2))
+= if (Seq.length input1 < l) then
+  ( () )
+  else
+  ( match parse p (Seq.slice input1 0 l), parse p (Seq.slice input2 0 l) with
+    | Some (v1, n1), Some (v2, n2) -> if n1 = l && n2 = l then
+                                      ( parser_kind_prop_equiv k p;
+                                        assert (injective_postcond p (Seq.slice input1 0 l) (Seq.slice input2 0 l)) )
+                                      else
+                                      ( () )
+    | _        -> () )
+
+let parse_exact_bare_injective
+  (#k: parser_kind)
+  (#t: Type0)
+  (p: parser k t)
+  (l: nat)
 : Lemma (
-  let a, len = x in
-  let sx = serialize (serialize_the_TL a) x in
-  let sx_T = serialize (serialize_the_asn1_tag a) a in
-  let sx_L = serialize serialize_asn1_length len in
-  sx == sx_T `Seq.append` sx_L /\
-  Seq.length sx == Seq.length sx_T + Seq.length sx_L)
-= parser_kind_prop_equiv (get_parser_kind (parse_the_asn1_tag a)) (parse_the_asn1_tag a);
-  parser_kind_prop_equiv (get_parser_kind parse_asn1_length) parse_asn1_length;
-  serialize_nondep_then_eq
-  (* s1 *) (serialize_the_asn1_tag a)
-  (* s2 *) (serialize_asn1_length)
-  (* in *) x
+  injective (parse_exact_bare p l)
+)
+= Classical.forall_intro_2 (
+    fun (s1 s2: bytes) ->
+      Classical.move_requires_2 (parse_exact_bare_injective_prf p l) s1 s2
+  )
 
-/// EverParse tagged union tag of asn1_value
-/// ASN.1 DER `Value` --> valid ASN.1 DER `Tag`, `Length` pair
-/// NOTE: Current considering 1) BOOLEAN: partial encoding; 2) NULL: empty; 3) OCTET_STRING: variable length
-///
-let parser_tag_of_the_asn1_value
-  (a: asn1_primitive_type)
-  (v: asn1_value_of_tag a)
-: Tot (parse_filter_refine (filter_the_TL a))
-= match a, v with
-  | BOOLEAN     , BOOLEAN_VALUE      b     -> (BOOLEAN     , 1ul)
-  | NULL        , NULL_VALUE        ()     -> (NULL        , 0ul)
-  | OCTET_STRING, OCTET_STRING_VALUE len s -> (OCTET_STRING, len)
+let parse_exact_kind
+  (#k: parser_kind)
+  (#t: Type0)
+  (p: parser k t)
+  (l: nat)
+: parser_kind = {
+  parser_kind_low = l;
+  parser_kind_high = Some l;
+  parser_kind_subkind = None;
+  parser_kind_metadata = None
+}
 
-// let parser_tag_of_asn1_value_impl
-//   (v: asn1_value)
-// : Tot (x: parse_filter_refine filter_TL{x == parser_tag_of_asn1_value v})
-// = match v with
-//   | BOOLEAN_VALUE      b   -> (BOOLEAN     , 1ul)
-//   | NULL_VALUE        ()   -> (NULL        , 0ul)
-//   | OCTET_STRING_VALUE l s -> (OCTET_STRING, U32.uint_to_t l)
-
-/// Synth functions
-let synth_the_asn1_boolean_value
-  (a: the_asn1_type BOOLEAN)
-  (x: parse_filter_refine (filter_the_TL a){x == (BOOLEAN, 1ul)})
-  (b: bool)
-: GTot (refine_with_tag (parser_tag_of_the_asn1_value a) x)
-= BOOLEAN_VALUE b
-
-let synth_the_asn1_boolean_value_inverse
-  (a: the_asn1_type BOOLEAN)
-  (x: parse_filter_refine (filter_the_TL a){x == (BOOLEAN, 1ul)})
-  (value: refine_with_tag (parser_tag_of_the_asn1_value a) x)
-: GTot bool
-= BOOLEAN_VALUE?.b value
-
-let synth_the_asn1_null_value
-  (a: the_asn1_type NULL)
-  (x: parse_filter_refine (filter_the_TL a){x == (NULL, 0ul)})
-  (n: unit)
-: GTot (refine_with_tag (parser_tag_of_the_asn1_value a) x)
-= NULL_VALUE n
-
-let synth_the_asn1_null_value_inverse
-  (a: the_asn1_type NULL)
-  (x: parse_filter_refine (filter_the_TL a){x == (NULL, 0ul)})
-  (value: refine_with_tag (parser_tag_of_the_asn1_value a) x)
-: GTot unit
-= NULL_VALUE?.n value
-
-let lbytes = Seq.Properties.lseq byte
-
-let synth_the_asn1_octet_string_value
-  (a: the_asn1_type OCTET_STRING)
-  (len: asn1_int32)
-  (x: parse_filter_refine (filter_the_TL a){x == (OCTET_STRING, len)})
-  (s: lbytes (U32.v len))
-: GTot (refine_with_tag (parser_tag_of_the_asn1_value a) x)
-= OCTET_STRING_VALUE len s
-
-let synth_the_asn1_octet_string_value_inverse
-  (a: the_asn1_type OCTET_STRING)
-  (len: asn1_int32)
-  (x: parse_filter_refine (filter_the_TL a){x == (OCTET_STRING, len)})
-  (value: refine_with_tag (parser_tag_of_the_asn1_value a) x)
-: GTot (s: lbytes (U32.v len))
-= OCTET_STRING_VALUE?.s value
-
-
-/// Strong parser kind for ASN.1 DER `Value` parser
-let parse_the_asn1_value_kind
-  (a: asn1_primitive_type)
-  (x: parse_filter_refine (filter_the_TL a))
-: parser_kind
-= let a, len = x in
-  let l = U32.v len in
-  strong_parser_kind l l None
-
-/// Weak Strong parser kind for ASN.1 DER `Value` parser, throw "runtime" tag, length
-let parse_asn1_value_kind_weak = strong_parser_kind asn1_length_min asn1_length_max None
-
-
-/// Parser for ASN.1 DER `Value`
-///
-let parse_the_asn1_value
-  (a: asn1_primitive_type)
-  (x: parse_filter_refine (filter_the_TL a))
-: Tot (parser (parse_the_asn1_value_kind a x) (refine_with_tag (parser_tag_of_the_asn1_value a) x))
-= let a, len = x in
-  let l: asn1_length_t = U32.v len in
-  match a with
-  | BOOLEAN      -> (parse_the_asn1_value_kind a x
-                     `weaken`
-                    (parse_asn1_boolean
-                     `parse_synth`
-                    // (fun b -> BOOLEAN_VALUE b <: refine_with_tag (parser_tag_of_the_asn1_value) x)
-                    (synth_the_asn1_boolean_value a x)))
-
-  | NULL         -> (parse_the_asn1_value_kind a x
-                     `weaken`
-                    (parse_asn1_null
-                     `parse_synth`
-                    // (fun n -> NULL_VALUE n <: refine_with_tag (parser_tag_of_the_asn1_value) x)
-                    (synth_the_asn1_null_value a x)))
-
-  | OCTET_STRING -> (parse_the_asn1_value_kind a x
-                     `weaken`
-                    (parse_asn1_octet_string l
-                     `parse_synth`
-                    // (fun (s: lbytes len) -> OCTET_STRING_VALUE s len <: refine_with_tag (parser_tag_of_the_asn1_value) x)
-                    (synth_the_asn1_octet_string_value a len x)))
-
-#push-options "--query_stats --z3rlimit 32 --max_fuel 16 --max_ifuel 16"
-let parse_the_asn1_value_unfold
-  (_a: asn1_primitive_type)
-  (x: parse_filter_refine (filter_the_TL _a))
-  (input: bytes)
+let parse_exact_correct
+  (#k: parser_kind)
+  (#t: Type0)
+  (p: parser k t)
+  (l: nat)
 : Lemma (
-  let a, len = x in
-  let l: asn1_length_t = U32.v len in
-  let value = parse (parse_the_asn1_value a x) input in
-  match a with
-  | BOOLEAN      -> (match parse parse_asn1_boolean input with
-                     | None -> value == None
-                     | Some (b, consumed) ->
-                            (parser_tag_of_the_asn1_value) a (BOOLEAN_VALUE b) == x /\
-                            consumed == l /\
-                            value == Some (BOOLEAN_VALUE b, consumed))
+  parser_kind_prop (parse_exact_kind p l) (parse_exact_bare p l)
+)
+= parser_kind_prop_equiv (parse_exact_kind p l) (parse_exact_bare p l);
+  parse_exact_bare_injective p l
 
-  | NULL         -> (match parse parse_asn1_null input with
-                     | None -> value == None
-                     | Some (null, consumed) ->
-                            (parser_tag_of_the_asn1_value) a (NULL_VALUE null) == x /\
-                            consumed == l /\
-                            value == Some (NULL_VALUE null, consumed))
+let parse_exact
+  (#k: parser_kind)
+  (#t: Type0)
+  (p: parser k t)
+  (l: nat)
+: parser (parse_exact_kind p l) t
+= parse_exact_correct p l;
+  parse_exact_bare p l
 
-  | OCTET_STRING -> (match parse (parse_asn1_octet_string l) input with
-                     | None -> value == None
-                     | Some (s, consumed) -> True \/
-                            (parser_tag_of_the_asn1_value) a (OCTET_STRING_VALUE len s) == x /\
-                            consumed == l /\
-                            value == Some (OCTET_STRING_VALUE len s, consumed)))
-= let a, len = x in
-  let l = U32.v len in
-  match a with
-  | BOOLEAN      -> (parse_asn1_boolean_unfold input;
-                     parser_kind_prop_equiv (get_parser_kind parse_asn1_boolean) parse_asn1_boolean;
-                     parse_synth_eq
-                     (* p1 *) (parse_asn1_boolean)
-                     (* f2 *) (synth_the_asn1_boolean_value a x)
-                           // (fun b -> BOOLEAN_VALUE b <: refine_with_tag (parser_tag_of_the_asn1_value) x)
-                     (* in *) input)
-
-  | NULL         -> (parse_synth_eq
-                     (* p1 *) (parse_asn1_null)
-                     (* f2 *) (synth_the_asn1_null_value a x)
-                           // (fun n -> NULL_VALUE n <: refine_with_tag (parser_tag_of_the_asn1_value) x)
-                     (* in *) input)
-
-  | OCTET_STRING -> (parse_synth_eq
-                     (* p1 *) (parse_asn1_octet_string l)
-                     (* f2 *) (synth_the_asn1_octet_string_value a len x)
-                           // (fun (s: lbytes len) -> OCTET_STRING_VALUE s len <: refine_with_tag (parser_tag_of_the_asn1_value) x)
-                     (* in *) input)
-
-/// Serializer for ASN.1 DER `Value`
+/// Example
 ///
-let serialize_the_asn1_value
-  (_a: asn1_primitive_type)
-  (x: parse_filter_refine (filter_the_TL _a))
-: Tot (serializer (parse_the_asn1_value _a x))
-= let a, len = x in
-  let l = U32.v len in
-  match a with
-  | BOOLEAN      -> (parse_the_asn1_value_kind a x
-                    `serialize_weaken`
-                    (serialize_synth
-                     (* p1 *) (parse_asn1_boolean)
-                     (* f2 *) (synth_the_asn1_boolean_value a x)
-                           // (fun b -> BOOLEAN_VALUE b <: refine_with_tag (parser_tag_of_the_asn1_value) x)
-                     (* s1 *) (serialize_asn1_boolean)
-                     (* g1 *) (synth_the_asn1_boolean_value_inverse a x)
-                           // (fun v -> BOOLEAN_VALUE?.b v)
-                     (* prf*) ()))
+type inner_t = {
+  n1: datatype_of_asn1_type NULL;
+  s1: datatype_of_asn1_type OCTET_STRING
+}
 
-  | NULL         -> (parse_the_asn1_value_kind a x
-                     `serialize_weaken`
-                    (serialize_synth
-                     (* p1 *) (parse_asn1_null)
-                     (* f2 *) (synth_the_asn1_null_value a x)
-                           // (fun n -> NULL_VALUE n <: refine_with_tag (parser_tag_of_the_asn1_value) x)
-                     (* s1 *) (serialize_asn1_null)
-                     (* g1 *) (synth_the_asn1_null_value_inverse a x)
-                           // (fun v -> NULL_VALUE?.n v)
-                     (* prf*) ()))
+let inner_t' = (
+  datatype_of_asn1_type NULL &
+  datatype_of_asn1_type OCTET_STRING
+)
 
-  | OCTET_STRING -> (parse_the_asn1_value_kind a x
-                     `serialize_weaken`
-                    (serialize_synth
-                     (* p1 *) (parse_asn1_octet_string l)
-                     (* f2 *) (synth_the_asn1_octet_string_value a len x)
-                     (* s1 *) (serialize_asn1_octet_string l)
-                     (* g1 *) (synth_the_asn1_octet_string_value_inverse a len x)
-                     (* prf*) ()))
+let synth_inner_t
+  (x': inner_t')
+: GTot (inner_t)
+= let n1, s1 = x' in
+  {n1 = n1; s1 = s1}
 
-let serialize_the_asn1_value_unfold
-  (_a: asn1_primitive_type)
-  (x: parse_filter_refine (filter_the_TL _a))
-  (value: refine_with_tag (parser_tag_of_the_asn1_value _a) x)
-: Lemma (
-  let a, len = x in
-  let l = U32.v len in
-  let sx = serialize (serialize_the_asn1_value a x) value in
-  match a with
-  | BOOLEAN      -> (sx == serialize serialize_asn1_boolean      (BOOLEAN_VALUE?.b value)      /\
-                     l == Seq.length sx)
-  | NULL         -> (sx == serialize serialize_asn1_null         (NULL_VALUE?.n value)         /\
-                     l == Seq.length sx)
-  | OCTET_STRING -> (sx == serialize (serialize_asn1_octet_string l) (OCTET_STRING_VALUE?.s value) /\
-                     l == Seq.length sx))
-= let a, len = x in
-  let l = U32.v len in
-  match a with
-  | BOOLEAN      -> (serialize_synth_eq
-                     (* p1 *) (parse_asn1_boolean)
-                     (* f2 *) (synth_the_asn1_boolean_value a x)
-                           // (fun b -> BOOLEAN_VALUE b <: refine_with_tag (parser_tag_of_the_asn1_value) a x)
-                     (* s1 *) (serialize_asn1_boolean)
-                     (* g1 *) (synth_the_asn1_boolean_value_inverse a x)
-                           // (fun v -> BOOLEAN_VALUE?.b v)
-                     (* prf*) ()
-                     (* x  *) (value))
+let synth_inner_t_inverse
+  (x: inner_t)
+: GTot (x': inner_t'{x == synth_inner_t x'})
+= (x.n1, x.s1)
 
-  | NULL         -> (serialize_synth_eq
-                     (* p1 *) (parse_asn1_null)
-                     (* f2 *) (synth_the_asn1_null_value a x)
-                           // (fun n -> NULL_VALUE n <: refine_with_tag (parser_tag_of_the_asn1_value) a x)
-                     (* s1 *) (serialize_asn1_null)
-                     (* g1 *) (synth_the_asn1_null_value_inverse a x)
-                           // (fun v -> NULL_VALUE?.n v)
-                     (* prf*) ()
-                     (* x  *) (value))
+let len_of_inner_t
+  (x: inner_t)
+: Tot (option (asn1_int32_of_tag SEQUENCE))
+= let len_n1 = len_of_asn1_primitive_TLV x.n1 in
+  let len_s1 = len_of_asn1_primitive_TLV x.s1 in
+  len_n1 `safe_add` len_s1
 
-  | OCTET_STRING -> (serialize_synth_eq
-                     (* p1 *) (parse_asn1_octet_string l)
-                     (* f2 *) (synth_the_asn1_octet_string_value a len x)
-                     (* s1 *) (serialize_asn1_octet_string l)
-                     (* g1 *) (synth_the_asn1_octet_string_value_inverse a len x)
-                     (* prf*) ()
-                     (* x  *) (value))
+let parse_inner
+: parser _ inner_t
+= parse_asn1_TLV_of_type NULL
+  `nondep_then`
+  parse_asn1_TLV_of_type OCTET_STRING
+  `parse_synth`
+  synth_inner_t
 
+let serialize_inner
+: serializer parse_inner
+= serialize_synth
+  (* p1 *) (parse_asn1_TLV_of_type NULL
+            `nondep_then`
+            parse_asn1_TLV_of_type OCTET_STRING)
+  (* f1 *) (synth_inner_t)
+  (* s1 *) (serialize_asn1_TLV_of_type NULL
+            `serialize_nondep_then`
+            serialize_asn1_TLV_of_type OCTET_STRING)
+  (* g1 *) (synth_inner_t_inverse)
+  (* Prf*) ()
 
-/// Kind for ASN.1 DER Tag, Length, Value tuple parser
-let parse_TLV_kind_of_tag
-  (_a: asn1_primitive_type)
-= get_parser_kind (parse_the_TL _a)
-  `and_then_kind`
-  parse_asn1_value_kind_weak
+let parse_exact_kind_weak = {
+  parser_kind_low = asn1_length_min;
+  parser_kind_high = Some asn1_length_max;
+  parser_kind_subkind = None;
+  parser_kind_metadata = None
+}
 
-/// Parser for ASN.1 DER Tag, Length, Value tuples
-///
-let parse_TLV_of_tag
-  (_a: asn1_primitive_type)
-: parser (parse_TLV_kind_of_tag _a) (asn1_value_of_tag _a)
-= parse_tagged_union
-    (parse_the_TL _a)
-    (parser_tag_of_the_asn1_value _a)
-    (fun x -> parse_asn1_value_kind_weak
+let parser_tag_of_sequence
+  (x: inner_t{Some? (len_of_inner_t x)})
+: GTot (the_asn1_type SEQUENCE * asn1_int32_of_tag SEQUENCE)
+= (SEQUENCE, (Some?.v (len_of_inner_t x)))
+
+let parse_inner_TLV
+= let p = (fun (x: (the_asn1_type SEQUENCE * asn1_int32_of_tag SEQUENCE)) ->
+            parse_exact_kind_weak
             `weaken`
-            parse_the_asn1_value _a x)
+            parse_exact parse_inner (I.v (snd x))) in
+  // assume (and_then_cases_injective p);
+  parse_tagged_union
+  (* pt *) (parse_the_asn1_tag SEQUENCE
+            `nondep_then`
+            parse_asn1_length_of_tag SEQUENCE)
+  (* tg *) (parser_tag_of_sequence)
+  (* p  *) (p)
 
-let parse_TLV_of_tag_unfold
-  (_a: asn1_primitive_type)
-  (input: bytes)
-: Lemma (
-  parse (parse_TLV_of_tag _a) input ==
-  (match parse (parse_the_TL _a) input with
-  | None -> None
-  | Some (x, consumed_TL) ->
-        (let input_value = Seq.slice input consumed_TL (Seq.length input) in
-         match (parse_the_asn1_value _a) x input_value with
-         | None -> None
-         | Some (value', consumed_v) -> Some (value', consumed_TL + consumed_v))))
-= parse_tagged_union_eq
-  (* pt *) (parse_the_TL _a)
-  (* tg *) ((parser_tag_of_the_asn1_value _a))
-  (* p  *) (fun x -> parse_asn1_value_kind_weak
-                   `weaken`
-                   (parse_the_asn1_value _a) x)
-  (* in *) (input)
+let serialize_inner_TLV
+= ()
 
-/// Serializer for ASN.1 DER Tag, Length, Value tuples
-///
-let serialize_TLV_of_tag
-  (_a: asn1_primitive_type)
-: serializer (parse_TLV_of_tag _a)
-= serialize_tagged_union
-    (serialize_the_TL _a)
-    (parser_tag_of_the_asn1_value _a)
-    (fun x -> parse_asn1_value_kind_weak
-            `serialize_weaken`
-            serialize_the_asn1_value _a x)
+type outer_t = {
+  b: datatype_of_asn1_type BOOLEAN;
+  inner: inner_t;
+  s: datatype_of_asn1_type OCTET_STRING
+}
 
-let serialize_TLV_of_tag_unfold
-  (_a: asn1_primitive_type)
-  (value: asn1_value_of_tag _a)
-: Lemma (
-  let x = (parser_tag_of_the_asn1_value _a) value in
-  let sx = serialize (serialize_TLV_of_tag _a) value in
-  let sx_TL = serialize (serialize_the_TL _a) x in
-  let sx_V  = serialize (serialize_the_asn1_value _a x) value in
-  sx == sx_TL `Seq.append` sx_V /\
-  Seq.length sx == Seq.length sx_TL + Seq.length sx_V)
-= let x = (parser_tag_of_the_asn1_value _a) value in
-  parser_kind_prop_equiv (get_parser_kind (parse_the_TL _a)) (parse_the_TL _a);
-  parser_kind_prop_equiv (get_parser_kind (parse_the_asn1_value _a x)) (parse_the_asn1_value _a x);
-  serialize_tagged_union_eq
-  (* st *) (serialize_the_TL _a)
-  (* tg *) ((parser_tag_of_the_asn1_value _a))
-  (* s  *) (fun x -> parse_asn1_value_kind_weak
-                   `serialize_weaken`
-                   serialize_the_asn1_value _a x)
-  (* in *) (value)
+(*)
+let len_of_outter_t
+  (x: outer_t)
+: Tot (option (asn1_int32_of_tag SEQUENCE))
+= let len_b = len_of_asn1_primitive_TLV x.b in
+  if (Some? len_b) then
+  ( let len_inner =  )
